src/ShouldBuild.v
@@ -21,8 +21,8 @@ From Perennial.program_proof.examples Require
      dir_proof
      single_inode_proof
      alloc_crash_proof
-     (* indirect_inode_proof
-     indirect_inode_append_proof *)
+     indirect_inode_proof
+     indirect_inode_append_proof
      replicated_block_proof
      toy_proof.
 From Perennial.goose_lang Require
